Use sections and notations in testing modules #149

base/coq/Free/Verification/SharingHandlerTests.v
@@ -32,59 +32,120 @@ Definition evalTracing {A : Type} p
 Definition evalNDM {A : Type} p
 := @collectVals (option A) (run (runChoice (runNDSharing (0,0) (runMaybe p)))).
 
-(* Shortcut to evaluate a traced partial program to a result and a list 
+(* Shortcut to evaluate a traced partial pro gram to a result and a list 
    of logged messages. *)
 Definition evalTraceM {A : Type} p
 := @collectMessages (option A) 
    (run (runTracing (runTraceSharing (0,0) (runMaybe p)))).
 
-(* Non-deterministic integer. *)
-Definition coin (Shape : Type) (Pos : Shape -> Type)
-                `{Injectable ND.Shape ND.Pos Shape Pos}
-:= Choice Shape Pos (pure 0%Z) (pure 1%Z).
-Arguments coin {_} {_} {_}.
+Section SecData.
 
+Variable Shape : Type.
+Variable Pos : Shape -> Type.
+
+Notation "'ND'" := (Injectable ND.Shape ND.Pos Shape Pos).
+Notation "'Trace'" := (Traceable Shape Pos).
+Notation "'Maybe'" := (Injectable Maybe.Shape Maybe.Pos Shape Pos).
+
+(* Non-deterministic integer. *)
+Definition coin `{ND}
+:= Choice Shape Pos (pure 0%Z) (pure 1%Z).
 
 (* Non-deterministic boolean value. *)
-Definition coinB (Shape : Type) (Pos : Shape -> Type)
-                 `{Injectable ND.Shape ND.Pos Shape Pos}
- := Choice Shape Pos (True_ _ _) (False_ _ _).
-Arguments coinB {_} {_} {_}.
+Definition coinB `{ND} := Choice Shape Pos (True_ _ _) (False_ _ _).
 
 (* Non-deterministic partial integer. *)
-Definition coinM (Shape : Type) (Pos : Shape -> Type)
-                 `{Injectable ND.Shape ND.Pos Shape Pos}
-                 `{Injectable Maybe.Shape Maybe.Pos Shape Pos}
+Definition coinM `{ND} `{Maybe} 
 := Choice Shape Pos (Nothing_inj _ _) (Just_inj _ _ 1%Z).
-Arguments coinM {_} {_} {_} {_}.
 
 (* Traced integer. *)
-Definition traceOne (Shape : Type) (Pos : Shape -> Type)
-                    `{Traceable Shape Pos}
-:= trace "One" (pure 1%Z).
-Arguments traceOne {_} {_} {_}.
+Definition traceOne `{Trace} := trace "One" (pure 1%Z).
 
 (* Traced boolean values. *)
-Definition traceTrue (Shape : Type) (Pos : Shape -> Type)
-                     `{Traceable Shape Pos}
-:= trace "True" (True_ _ _).
-Arguments traceTrue {_} {_} {_}.
-Definition traceFalse (Shape : Type) (Pos : Shape -> Type)
-                      `{Traceable Shape Pos}
-:= trace "False" (False_ _ _).
-Arguments traceFalse {_} {_} {_}.
+Definition traceTrue `{Trace} := trace "True" (True_ _ _).
+
+Definition traceFalse `{Trace} := trace "False" (False_ _ _).
 
 (* Traced Maybe values *)
-Definition traceNothing (Shape : Type) (Pos : Shape -> Type)
-                        `{Traceable Shape Pos}
-                        `{Injectable Maybe.Shape Maybe.Pos Shape Pos}
+Definition traceNothing `{Trace} `{Maybe}
 := trace "Nothing" (@Nothing_inj (Integer Shape Pos) _ _ _).
+
+Definition traceJust `{Trace} `{Maybe} := trace "Just 1" (Just_inj _ _ 1%Z).
+
+End SecData.
+
+(* Arguments sentences for the data. *)
+Arguments coin {_} {_} {_}.
+Arguments coinB {_} {_} {_}.
+Arguments coinM {_} {_} {_} {_}.
+Arguments traceOne {_} {_} {_}.
+Arguments traceTrue {_} {_} {_}.
+Arguments traceFalse {_} {_} {_}.
 Arguments traceNothing {_} {_} {_} {_}.
-Definition traceJust (Shape : Type) (Pos : Shape -> Type)
-                     `{Traceable Shape Pos}
-                     `{Injectable Maybe.Shape Maybe.Pos Shape Pos}
-:= trace "Just 1" (Just_inj _ _ 1%Z).
 Arguments traceJust {_} {_} {_} {_}.
+
+(* Test functions *)
+Section SecFunctions.
+
+Set Implicit Arguments.
+Variable Shape : Type.
+Variable Pos : Shape -> Type.
+Variable A : Type.
+Notation "'FreeA'" := (Free Shape Pos A).
+Notation "'ShareArgs'" := (ShareableArgs Shape Pos A).
+
+(* This function applies the given binary function to the given argument
+   twice and does not share the argument. *)
+Definition double (f : FreeA -> FreeA -> FreeA ) (fx : FreeA) : FreeA
+:= f fx fx.
+
+(* Simple sharing: 
+   let sx = fx in f sx sx *)
+Definition doubleShared `(Shareable Shape Pos) `{ShareArgs} 
+                        (f : FreeA -> FreeA -> FreeA)
+                        (fx : FreeA)
+ : FreeA
+:= share fx >>= fun sx => f sx sx.
+
+(* Nested sharing:
+   let sx = fx 
+       sy = f sx sx
+   in f sy sy *)
+Definition doubleSharedNested `(Shareable Shape Pos) `{ShareArgs}
+                              (f : FreeA -> FreeA -> FreeA)
+                              (fx : FreeA)
+ : FreeA
+:= share (share fx >>= fun sx => f sx sx) >>= fun sy =>
+   f sy sy.
+
+(* let sx = fx  
+       sy = f sx sx
+       sz = fy
+   in f sy sz *)
+Definition doubleSharedClash `(Shareable Shape Pos) `{ShareArgs}
+                             (f : FreeA -> FreeA -> FreeA)
+                             (fx : FreeA) (fy : FreeA)
+ : FreeA
+:= share (share fx >>= fun sx => f sx sx) >>= fun sy =>
+   share fy >>=  fun sz => f sy sz.
+
+(*
+let sx = val
+    sy = f sx fx
+    sz = f sy fy
+in f sx (f (sy (f sz val))) 
+*)
+Definition doubleSharedRec `(Shareable Shape Pos) `{ShareArgs}
+                           (f : FreeA -> FreeA -> FreeA)
+                           (fx : FreeA) (fy : FreeA)
+                           (val : A)
+ : FreeA
+:= share (pure val) >>= fun sx =>
+   f sx (share (f sx fx) >>= fun sy => 
+   f sy (share (f sy fy) >>= fun sz =>
+   f sz (pure val))).
+
+End SecFunctions.
 
 (* Some notations for convenience.
    Since we only provide the sharing instance and functions when the handlers
@@ -96,24 +157,12 @@ Notation "'orBool_'" := (orBool _ _).
 
 (* ---------------------- Test cases without sharing ----------------------- *)
 
-(* This function applies the given binary function to the given argument
-   twice and does not share the argument. *)
-Definition double {Shape : Type}
-                  {Pos : Shape -> Type}
-                  {A : Type}
-                  (f : Free Shape Pos A ->
-                       Free Shape Pos A -> 
-                       Free Shape Pos A)
-                  (fx : Free Shape Pos A)
- : Free Shape Pos A
-:= f fx fx.
-
 (* 
 0?1 + 0?1
 = 0+0 ? 0+1 ? 1+0 ? 1+1
 = 0 ? 1 ? 1 ? 2
 *)
-Example exAddNoSharingND : evalND (nf (double (addInteger_) coin))
+Example exAddNoSharingND : evalND (nf (double addInteger_ coin))
                            = [0%Z;1%Z;1%Z;2%Z].
 Proof. constructor. Qed.
 
@@ -122,7 +171,7 @@ trace "One" 1 + trace "One" 1
 => The message should be logged twice and the result should be 2.
 *)
 Example exAddNoSharingTrace 
-: evalTracing (nf (double (addInteger_) traceOne))
+: evalTracing (nf (double addInteger_ traceOne))
   = (2%Z,["One"%string;"One"%string]).
 Proof. constructor. Qed.
 
@@ -133,7 +182,7 @@ Proof. constructor. Qed.
 = true ? true ? false
 *)
 Example exOrNDNoSharing 
- : evalND (nf (double (orBool_) coinB)) = [true;true;false].
+ : evalND (nf (double orBool_ coinB)) = [true;true;false].
 Proof. constructor. Qed.
 
 (*
@@ -142,7 +191,7 @@ Proof. constructor. Qed.
    message should be logged only once.
 *)
 Example exOrTrueTracingNoSharing 
- : evalTracing (nf (double (orBool_) traceTrue))
+ : evalTracing (nf (double orBool_ traceTrue))
    = (true,["True"%string]).
 Proof. constructor. Qed.
 
@@ -152,7 +201,7 @@ Proof. constructor. Qed.
    should be logged twice.
 *)
 Example exOrFalseTracingNoSharing 
- : evalTracing (nf (double (orBool_) traceFalse))
+ : evalTracing (nf (double orBool_ traceFalse))
    = (false,["False"%string;"False"%string]).
 Proof. constructor. Qed.
 
@@ -174,7 +223,7 @@ Proof. constructor. Qed.
 = Nothing ? Nothing ? Just 2
 *)
 Example exNDMNoSharing
- : evalNDM (nf (double (addInteger_) coinM)) = [None;None;Some 2%Z].
+ : evalNDM (nf (double addInteger_ coinM)) = [None;None;Some 2%Z].
 Proof. constructor. Qed.
 
 (* 
@@ -183,7 +232,7 @@ trace "Nothing" Nothing + trace "Nothing" Nothing
    only be logged once and the result should be Nothing (i.e. None in Coq).
 *)
 Example exTraceNothingNoSharing
- : evalTraceM (nf (double (addInteger_) traceNothing))
+ : evalTraceM (nf (double addInteger_ traceNothing))
    = (None,["Nothing"%string]).
 Proof. constructor. Qed.
 
@@ -193,23 +242,12 @@ trace "Just 1" (Just 1) + trace "Just 1" (Just 1)
    result should be Just 2 (Some 2 in Coq).
 *)
 Example exTraceJustNoSharing
- : evalTraceM (nf (double (addInteger_) traceJust))
+ : evalTraceM (nf (double addInteger_ traceJust))
    = (Some 2%Z,["Just 1"%string;"Just 1"%string]).
 Proof. constructor. Qed.
 
+
 (* --------------------- Test cases for simple sharing --------------------- *)
-(* let sx = fx in f sx sx *)
-Definition doubleShared {Shape : Type}
-                        {Pos : Shape -> Type}
-                        {A : Type}
-                        `(S : Shareable Shape Pos)
-                        `{ShareableArgs Shape Pos A}
-                        (f : Free Shape Pos A ->
-                             Free Shape Pos A -> 
-                             Free Shape Pos A)
-                        (fx : Free Shape Pos A)
- : Free Shape Pos A
-:= share fx >>= fun sx => f sx sx.
 
 (*
 let sx = 0 ? 1 
@@ -218,7 +256,7 @@ in sx + sx
 = 0 ? 2
 *)
 Example exAddSharingND : evalND (nf (doubleShared Cbneed_
-  (addInteger_) coin))
+  addInteger_ coin))
   = [0%Z;2%Z].
 Proof. constructor. Qed.
 
@@ -228,7 +266,7 @@ in sx + sx
 => The message should be logged once and the result should be 2.
 *)
 Example exAddSharingTrace 
- : evalTracing (nf (doubleShared Cbneed_ (addInteger_) traceOne))
+ : evalTracing (nf (doubleShared Cbneed_ addInteger_ traceOne))
  = (2%Z,["One"%string]).
 Proof. constructor. Qed.
 
@@ -239,7 +277,7 @@ in sx or sx
 = true ? false
 *)
 Example exOrNDSharing
- : evalND (nf (doubleShared Cbneed_ (orBool_) coinB)) = [true;false].
+ : evalND (nf (doubleShared Cbneed_ orBool_ coinB)) = [true;false].
 Proof. constructor. Qed.
 
 (*
@@ -249,7 +287,7 @@ in sx or sx
    The message should be logged once and the result should be true.
 *)
 Example exOrTrueTraceSharing
- : evalTracing (nf (doubleShared (Cbneed_) (orBool_) traceTrue))
+ : evalTracing (nf (doubleShared Cbneed_ orBool_ traceTrue))
    = (true,["True"%string]).
 Proof. constructor. Qed.
 
@@ -260,7 +298,7 @@ in sx or sx
 only be logged once and the result should be false.
 *)
 Example exOrFalseTraceSharing
- : evalTracing (nf (doubleShared (Cbneed_) (orBool_) traceFalse))
+ : evalTracing (nf (doubleShared Cbneed_ orBool_ traceFalse))
    = (false,["False"%string]).
 Proof. constructor. Qed.
 
@@ -279,7 +317,7 @@ in sx + sx
 = Nothing ? Just 2
 *)
 Example exNDMSharing
- : evalNDM (nf (doubleShared (Cbneed_) (addInteger_) coinM))
+ : evalNDM (nf (doubleShared Cbneed_ addInteger_ coinM))
    = [None;Some 2%Z].
 Proof. constructor. Qed.
 
@@ -290,7 +328,7 @@ in sx + sx
    due to >>=.
 *)
 Example exTraceNothingSharing
- : evalTraceM (nf (doubleShared (Cbneed_) (addInteger_) traceNothing))
+ : evalTraceM (nf (doubleShared Cbneed_ addInteger_ traceNothing))
    = (None,["Nothing"%string]).
 Proof. constructor. Qed.
 
@@ -301,27 +339,11 @@ in sx + sx
    should be Some 2.
 *)
 Example exTraceJustSharing
- : evalTraceM (nf (doubleShared (Cbneed_) (addInteger_) traceJust))
+ : evalTraceM (nf (doubleShared Cbneed_ addInteger_ traceJust))
    = (Some 2%Z,["Just 1"%string]).
 Proof. constructor. Qed.
 
 (* --------------------- Test cases for nested sharing --------------------- *)
-
-(* let sx = fx 
-       sy = f sx sx
-   in f sy sy *)
-Definition doubleSharedNested {Shape : Type}
-                              {Pos : Shape -> Type}
-                              {A : Type}
-                              `(S : Shareable Shape Pos)
-                              `{ShareableArgs Shape Pos A}
-                              (f : Free Shape Pos A ->
-                                  Free Shape Pos A -> 
-                                  Free Shape Pos A)
-                                  (fx : Free Shape Pos A)
- : Free Shape Pos A
-:= share (share fx >>= fun sx => f sx sx) >>= fun sy =>
-   f sy sy.
 
 (* 
 let sx = 0 ? 1 
@@ -330,8 +352,8 @@ in sy + sy
 = (0+0)+(0+0) ? (1+1)+(1+1) 
 = 0 ? 4 
 *)
-Example exAddNestedSharingND : evalND (nf (doubleSharedNested (Cbneed_)
-                                                          (addInteger_) 
+Example exAddNestedSharingND : evalND (nf (doubleSharedNested Cbneed_
+                                                          addInteger_ 
                                                           coin))
                                = [0%Z;4%Z].
 Proof. constructor. Qed.
@@ -343,7 +365,7 @@ in sy + sy
 => The message should only be logged once and the result should be 4. 
 *)
 Example exAddNestedSharingTrace 
- : evalTracing (nf (doubleSharedNested (Cbneed_) (addInteger_) traceOne))
+ : evalTracing (nf (doubleSharedNested Cbneed_ addInteger_ traceOne))
    = (4%Z,["One"%string]).
 Proof. constructor. Qed.
 
@@ -354,7 +376,7 @@ in sy or sy
 = true ? false
 *)
 Example exOrNestedSharingND
- : evalND (nf (doubleSharedNested (Cbneed_) (orBool_) coinB))
+ : evalND (nf (doubleSharedNested Cbneed_ orBool_ coinB))
    = [true;false].
 Proof. constructor. Qed.
 
@@ -366,7 +388,7 @@ in sy or sy
    and the result should be true.
 *)
 Example exOrNestedTrueTracing 
- : evalTracing (nf (doubleSharedNested (Cbneed_) (orBool_) traceTrue))
+ : evalTracing (nf (doubleSharedNested Cbneed_ orBool_ traceTrue))
    = (true,["True"%string]).
 Proof. constructor. Qed.
 
@@ -378,27 +400,9 @@ in sy or sy
    and the result should be false.
 *)
 Example exOrNestedFalseTracing
- : evalTracing (nf (doubleSharedNested (Cbneed_) (orBool_) traceFalse))
+ : evalTracing (nf (doubleSharedNested Cbneed_ orBool_ traceFalse))
    = (false, ["False"%string]).
 Proof. constructor. Qed.
-
-(* let sx = fx  
-       sy = f sx sx
-       sz = fy
-   in f sy sz *)
-Definition doubleSharedClash {Shape : Type}
-                             {Pos : Shape -> Type}
-                             {A : Type}
-                             `(S : Shareable Shape Pos)
-                             `{ShareableArgs Shape Pos A}
-                             (f : Free Shape Pos A ->
-                                  Free Shape Pos A -> 
-                                  Free Shape Pos A)
-                             (fx : Free Shape Pos A)
-                             (fy : Free Shape Pos A)
- : Free Shape Pos A
-:= share (share fx >>= fun sx => f sx sx) >>= fun sy =>
-   share fy >>=  fun sz => f sy sz.
 
 (* 
 let sx = 0 ? 1
@@ -411,7 +415,7 @@ in sy + sz
 = 0 ? 1 ? 2 ? 3
 *)
 Example exAddClashSharingND
- : evalND (nf (doubleSharedClash (Cbneed_) (addInteger_) coin coin))
+ : evalND (nf (doubleSharedClash Cbneed_ addInteger_ coin coin))
    = [0%Z;1%Z;2%Z;3%Z].
 Proof. constructor. Qed.
 
@@ -423,7 +427,7 @@ in sy + sz
 => The message should be logged twice and the result should be 3.
 *)
 Example exAddClashSharingTracing
- : evalTracing (nf (doubleSharedClash (Cbneed_) (addInteger_)
+ : evalTracing (nf (doubleSharedClash Cbneed_ addInteger_
                                   traceOne traceOne))
    = (3%Z,["One"%string;"One"%string]).
 Proof. constructor. Qed.
@@ -438,7 +442,7 @@ in sy or sz
 = true ? true ? false
 *)
 Example exOrClashSharingND
- : evalND (nf (doubleSharedClash (Cbneed_) (orBool_) coinB coinB))
+ : evalND (nf (doubleSharedClash Cbneed_ orBool_ coinB coinB))
    = [true;true;false].
 Proof. constructor. Qed.
 
@@ -451,7 +455,7 @@ in sy or sz
    result should be true.
 *)
 Example exOrClashTrueTracing
- : evalTracing (nf (doubleSharedClash (Cbneed_) (orBool_)
+ : evalTracing (nf (doubleSharedClash Cbneed_ orBool_
                                   traceTrue traceTrue))
    = (true,["True"%string]).
 Proof. constructor. Qed.
@@ -466,35 +470,10 @@ in sy or sz
    be logged twice in total and the result should be false.
 *)
 Example exOrClashFalseTracing
- : evalTracing (nf (doubleSharedClash (Cbneed_) (orBool_)
+ : evalTracing (nf (doubleSharedClash Cbneed_ orBool_
                                   traceFalse traceFalse))
    = (false,["False"%string;"False"%string]).
 Proof. constructor. Qed.
-
-(*
-let sx = val
-    sy = f sx fx
-    sz = f sy fy
-in f sx (f (sy (f sz val))) 
-*)
-Definition doubleSharedRec {Shape : Type}
-                           {Pos : Shape -> Type}
-                           {A : Type}
-                           `(S : Shareable Shape Pos)
-                           `{ShareableArgs Shape Pos A}
-                           (f : Free Shape Pos A ->
-                                Free Shape Pos A -> 
-                                Free Shape Pos A)
-                           (fx : Free Shape Pos A)
-                           (fy : Free Shape Pos A)
-                           (val : A)
- : Free Shape Pos A
-:= share (pure val) >>= fun sx =>
-   f sx (share (f sx fx) >>= fun sy => 
-      f sy (share (f sy fy) >>= fun sz =>
-        f sz (pure val)
-      )
-   ).
 
 (*
 let sx = 1
@@ -508,8 +487,8 @@ in sx + (sy + (sz + 1))
   ? (1 + (1+1 + ((1+1 + 1) + 1)))
 = 4 ? 5 ? 6 ? 7
 *)
-Example exAddRecSharingND : evalND (nf (doubleSharedRec (Cbneed_)
-                                                    (addInteger_)
+Example exAddRecSharingND : evalND (nf (doubleSharedRec Cbneed_
+                                                    addInteger_
                                                     coin coin 1%Z))
                             = [4%Z;5%Z;6%Z;7%Z].
 Proof. constructor. Qed.
@@ -525,7 +504,7 @@ in sx + (sy + (sz + 1))
    final value should be 1 + 2 + 3 + 1 = 7.
 *)
 Example exAddRecSharingTracing
- : evalTracing (nf (doubleSharedRec (Cbneed_) (addInteger_)
+ : evalTracing (nf (doubleSharedRec Cbneed_ addInteger_
                                 traceOne traceOne 1%Z))
    = (7%Z,["One"%string;"One"%string]).
 Proof. constructor. Qed.
@@ -538,7 +517,7 @@ in sx or (sy or (sz or true))
 = true (due to non-strictness)
 *)
 Example exOrRecSharingNDTrue
- : evalND (nf (doubleSharedRec (Cbneed_) (orBool_) coinB coinB true))
+ : evalND (nf (doubleSharedRec Cbneed_ orBool_ coinB coinB true))
    = [true].
 Proof. constructor. Qed.
 
@@ -561,7 +540,7 @@ in sx or (sy or (sz or false))
 = true ? true ? false
 *)
 Example exOrRecSharingNDFalse
- : evalND (nf ((doubleSharedRec (Cbneed_) (orBool_) coinB coinB false)))
+ : evalND (nf ((doubleSharedRec Cbneed_ orBool_ coinB coinB false)))
    = [true;true;false].
 Proof. constructor. Qed.
 
@@ -574,7 +553,7 @@ in sx or (sy or (sz or false))
    be logged once and the result should be true.
 *)
 Example exOrRecTrueTracing
- : evalTracing (nf (doubleSharedRec (Cbneed_) (orBool_)
+ : evalTracing (nf (doubleSharedRec Cbneed_ orBool_
                                 traceTrue traceTrue false))
    = (true,["True"%string]).
 Proof. constructor. Qed.
@@ -589,8 +568,7 @@ in sx or (sy or (sz or false))
    be false.
 *)
 Example exOrRecFalseTracing
- : evalTracing (nf (doubleSharedRec (Cbneed_) (orBool_)
+ : evalTracing (nf (doubleSharedRec Cbneed_ orBool_
                                 traceFalse traceFalse false))
    = (false,["False"%string;"False"%string]).
 Proof. constructor. Qed.
-
